refactored sec chan with mask (xor-like) function

theories/prob_eff_lang/probblaze/examples/DH_KE/mask_bijection.v
@@ -1,6 +1,6 @@
 From iris.proofmode Require Import base.
 From mathcomp Require all_boot ssrnat prime solvable.cyclic.
-From clutch.prelude Require base.
+From clutch.prelude Require base classical.
 From clutch.prob_eff_lang.probblaze.examples.DH_KE Require valgroup mask.
 From Stdlib Require Import Lia.
 Set Default Proof Using "Type*".
@@ -10,6 +10,7 @@ Section sc_bijection.
   Import prime fingroup ssralg (* all_boot *) zmodp valgroup mask base stdpp_ext.
   Import GroupScope. (* For group-related notations *)
   Import GRing.Theory. (* For ring-related notations like + and * *)
+  Import classical.
   Open Scope ring_scope.
   Context `{logic.probblazeRGS Σ}.
   Context {vg: val_group}.
@@ -17,7 +18,7 @@ Section sc_bijection.
   Context {G : clutch_group (vg:=vg) (cg:=cg)}.
   Context {vgg : @val_group_generator vg}.
   #[local] Notation n := (S (S n'')).
-  Context {mask_struct : @Mask (@vgG vg)}.
+  Context {mask_struct : @Mask (@vgG vg) (vgval)}.
   Context `{!Mask_struc}.
 
   Lemma g_log_exp (x : Fin.t n) : g_log (g ^+ fin.fin_to_nat x)%g = x.
@@ -45,30 +46,40 @@ Section sc_bijection.
       apply bij_surj.
   Qed.       
 
-  Definition sc_coupling_nat (m : vgG) : nat -> nat := fun (k : nat) => match (decide (k < n)) with
-                                                                        | left H => fin.fin_to_nat (sc_coupling_fin m (nat_to_fin H))
-                                                                        | right _ => k
-                                                                        end .
+  Definition sc_coupling_nat (m : vgG) : nat -> nat := fun (k : nat) => if (decide (k < n)) then g_log (f_inv (λ x, mask_sem x m) (g ^+ k)%g) else k.
 
   Global Instance sc_coupling_nat_bij (m : vgG) : Bij (sc_coupling_nat m).
   Proof.
     split. 
     - intros x y Heq. unfold sc_coupling_nat in Heq. 
         case_decide as Hx; case_decide as Hy; last done.
-        + repeat apply (inj _) in Heq. 
+        + destruct (f_inv_bij (λ x : vgG, mask_sem x m))  as [Hinj _].
+          repeat apply (inj _) in Heq. 
+          rewrite -(fin_to_nat_to_fin x n Hx) -(fin_to_nat_to_fin y n Hy) in Heq.
+          apply (inj (λ x, (g ^+ fin.fin_to_nat x)%g)) in Heq.
           apply (f_equal fin_to_nat) in Heq. 
           by rewrite !fin_to_nat_to_fin in Heq. 
         + subst. exfalso. eauto using fin_to_nat_lt.
         + subst. exfalso. eauto using fin_to_nat_lt.
       - intros k. unfold sc_coupling_nat.
         destruct (decide (k < S (S n''))%nat) as [Hk | Hk]; try (exists k; case_decide; done).
-        destruct (surj (sc_coupling_fin m) (nat_to_fin Hk)) as [i Hi].
-        exists (fin_to_nat i).
-        case_decide as Hi'; [| pose proof (fin_to_nat_lt i); lia].
-        rewrite -(fin_to_nat_to_fin _ _ Hk).
-        rewrite -Hi. by rewrite nat_to_fin_to_nat.
+        destruct (surj g_log (nat_to_fin Hk)) as [k1 Hk1].  
+        destruct (f_inv_bij (λ x : vgG, mask_sem x m))  as [_ Hfsurj].
+        destruct (surj (f_inv (λ x0, mask_sem x0 m)) k1) as [k2 Hk2].
+        destruct (surj (λ x : fin n, (g ^+ x)%g) k2) as [k3 Hk3].
+        exists (fin_to_nat k3). case_decide.
+        + by rewrite Hk3 Hk2 Hk1 fin_to_nat_to_fin.
+        + exfalso. apply H1. apply fin_to_nat_lt.  
   Qed.    
-    
+
+  Lemma sc_coupling_nat_bound m :  ∀ k : nat, (k < S (S n''))%nat → (sc_coupling_nat m k < S (S n''))%nat.
+  Proof. 
+    intros k Hlt.
+    unfold sc_coupling_nat.
+    case_decide; last done.
+    apply fin_to_nat_lt.
+  Qed. 
+
   Lemma sc_coupling_mask (m : vgG) (x : Fin.t n) :
     (g ^+ fin.fin_to_nat (sc_coupling_fin m x))%g = mask_sem (g ^+ fin.fin_to_nat x)%g m.
   Proof.
@@ -81,24 +92,31 @@ Section sc_bijection.
   Proof.
     unfold sc_coupling_fin.
     rewrite !sc_coupling_mask.
-    by rewrite mask_masklutive.
+    by rewrite mask_involutive.
   Qed.
   
-  (* I don't think we need this lemma *)
-  (* Lemma sc_coupling_involutive (m : vgG) : Involutive eq (sc_coupling_fin m).
-     Proof.
-       intros x. unfold sc_coupling_fin.
-       rewrite sc_coupling_mask. 
-       rewrite mask_bij.
-       destruct g_exp_bij as [Hg _]. apply Hg.
-       apply int_of_vg_sem_inj.
-       rewrite !int_sc_coupling.
-       apply xor_sem_invol.
-       - pose proof (int_of_vg_sem_bound m) as Hb. rewrite vgG_card in Hb. lia.
-       - pose proof (int_of_vg_sem_bound (g ^+ fin.fin_to_nat x)%g) as Hb.
-         rewrite vgG_card in Hb. lia.
-     Qed. *)
-  
+  Lemma sc_coupling_nat_mask (m : vgG) (x : nat) : 
+    (x < n) → 
+    (g ^+ x)%g = mask_sem (g ^+ (sc_coupling_nat m x))%g m.
+  Proof. 
+    intros Hlt.
+    unfold sc_coupling_nat. case_decide; last lia.
+    rewrite g_log_id.
+    by rewrite (f_inv_cancel_r (λ x, mask_sem x m)).
+  Qed. 
+
+  Lemma sc_coupling_nat_invol (m : vgG) (x : nat) :
+    (x < n) →
+    m = mask_sem (g ^+ (sc_coupling_nat m x))%g (g ^+ x)%g.
+  Proof. 
+    intros Hlt.
+    unfold sc_coupling_nat.
+    case_decide; last lia.
+    rewrite g_log_id.
+    rewrite (sc_coupling_nat_mask m); last done.
+    rewrite (f_inv_cancel_l (λ x, mask_sem x m)).
+    by rewrite mask_involutive.
+  Qed. 
   
   (* [g_log_exp] for a nat exponent.  Needed where the index is a [nat]
      carrying a separate bound rather than a [Fin.t n] -- e.g. proofs that go
